doc-src/TutorialI/Misc/cases.thy
@@ -5,11 +5,13 @@ theory "cases" = Main:;
 lemma "(case xs of [] \\<Rightarrow> [] | y#ys \\<Rightarrow> xs) = xs";
 apply(case_tac xs);
 
-txt{*
+txt{*\noindent
+results in the proof state
 \begin{isabellepar}%
 ~1.~xs~=~[]~{\isasymLongrightarrow}~(case~xs~of~[]~{\isasymRightarrow}~[]~|~y~\#~ys~{\isasymRightarrow}~xs)~=~xs\isanewline
 ~2.~{\isasymAnd}a~list.~xs=a\#list~{\isasymLongrightarrow}~(case~xs~of~[]~{\isasymRightarrow}~[]~|~y\#ys~{\isasymRightarrow}~xs)~=~xs%
 \end{isabellepar}%
+which is solved automatically:
 *}
 
 apply(auto).;
