doc-src/TutorialI/Trie/Option2.thy
@@ -2,8 +2,7 @@
 theory Option2 = Main:;
 (*>*)
 
-datatype 'a option = None | Some 'a
-
+datatype 'a option = None | Some 'a;
 (*<*)
 end
 (*>*)
